Adjustment of C code, discovery of some pq constraints, adjustments to invariant

prim/spatial_undirected_matrix.v
@@ -22,16 +22,73 @@ Proof. unfold SIZE. set (i:=Int.max_signed); compute in i; subst i. lia. Qed.
 
 Definition inf := Int.max_signed - Int.max_signed / SIZE.
 
+Lemma inf_rep: 0 <= inf < Int.max_signed.
+Proof. unfold inf. set (i:=Int.max_signed); compute in i; subst i. unfold SIZE.
+set (j:=2147483647 / 8); compute in j; subst j. lia. Qed.
+
 Definition G := @MatrixUGraph inf SIZE.
-Definition edgeless_graph_SIZE := @edgeless_graph inf SIZE SIZE_rep.
+Definition edgeless_graph' := @edgeless_graph inf SIZE inf_rep SIZE_rep.
 
 Definition eformat (e: E) := if fst e <=? snd e then e else (snd e, fst e).
 
 Lemma eformat1: forall (e: E), fst e <= snd e -> eformat e = e.
 Proof. unfold eformat; intros. rewrite Zle_is_le_bool in H; rewrite H. auto. Qed.
 
-Lemma eformat2: forall (e: E), snd e < fst e -> eformat e = (snd e, fst e).
+Lemma eformat2': forall (e: E), snd e < fst e -> eformat e = (snd e, fst e).
 Proof. unfold eformat; intros. rewrite <- Z.leb_gt in H; rewrite H. auto. Qed.
+
+Lemma eformat2: forall (e: E), snd e <= fst e -> eformat e = (snd e, fst e).
+Proof.
+intros. apply Z.le_lteq in H. destruct H. rewrite eformat2'; auto. rewrite eformat1, H. rewrite <- H at 2. destruct e; auto. lia.
+Qed.
+
+Lemma eformat_symm:
+forall u v, eformat (u,v) = eformat (v,u).
+Proof.
+intros. destruct (Z.lt_trichotomy u v).
+rewrite eformat1. rewrite eformat2. simpl; auto. simpl; lia. simpl; lia.
+destruct H.
+rewrite eformat1. rewrite eformat2. simpl; auto. simpl; lia. simpl; lia.
+rewrite eformat2'. rewrite eformat1. simpl; auto. simpl; lia. simpl; lia.
+Qed.
+
+Lemma eformat_adj: forall (g: G) u v, adjacent g u v <-> elabel g (eformat (u,v)) <> inf.
+Proof.
+intros. pose proof (@edge_weight_not_inf _ _ _ (sound_MatrixUGraph g)).
+split; intros.
++
+destruct H0. destruct H0. destruct H0.
+destruct H1; destruct H1. assert (x = (u,v)). {
+  rewrite (@src_fst _ _ _ (sound_MatrixUGraph g) x H0) in H1.
+  rewrite (@dst_snd _ _ _ (sound_MatrixUGraph g) x H0) in H3. rewrite <- H1, <- H3. destruct x; simpl; auto.
+} subst x.
+rewrite eformat1. apply H; auto. simpl; auto.
+rewrite <- H1. rewrite <- H3 at 2. apply (@undirected_edge_rep _ _ _ (sound_MatrixUGraph g)). auto.
+assert (x = (v,u)). {
+  rewrite (@src_fst _ _ _ (sound_MatrixUGraph g) x H0) in H1.
+  rewrite (@dst_snd _ _ _ (sound_MatrixUGraph g) x H0) in H3. rewrite <- H1, <- H3. destruct x; simpl; auto.
+} subst x.
+rewrite eformat2. simpl. apply H; auto. simpl. rewrite <- H1. rewrite <- H3 at 2.
+apply (@undirected_edge_rep _ _ _ (sound_MatrixUGraph g)). auto.
++
+destruct (Z.lt_trichotomy u v).
+rewrite eformat1 in H0. 2: simpl; lia.
+assert (evalid g (u,v)). apply evalid_inf_iff; auto.
+exists (u,v). split. apply evalid_strong_evalid; auto. left.
+rewrite (@src_fst _ _ _ (sound_MatrixUGraph g)); auto.
+rewrite (@dst_snd _ _ _ (sound_MatrixUGraph g)); auto.
+(*equal, repeat*)
+destruct H1. rewrite eformat1 in H0. 2: simpl; lia.
+assert (evalid g (u,v)). apply evalid_inf_iff; auto.
+exists (u,v). split. apply evalid_strong_evalid; auto. left.
+rewrite (@src_fst _ _ _ (sound_MatrixUGraph g)); auto.
+rewrite (@dst_snd _ _ _ (sound_MatrixUGraph g)); auto.
+rewrite eformat2 in H0. 2: simpl; lia. simpl in H0.
+assert (evalid g (v,u)). apply evalid_inf_iff; auto.
+exists (v,u). split. apply evalid_strong_evalid; auto.
+rewrite (@src_fst _ _ _ (sound_MatrixUGraph g)); auto.
+rewrite (@dst_snd _ _ _ (sound_MatrixUGraph g)); auto.
+Qed.
 
 (*When these are unfolded in the goal and I destruct evalid_dec, I can get the hypothesis but the if... doesn't simplify
 
@@ -47,14 +104,23 @@ Definition vert_rep_symm (g : G) (v : V): list Z :=
 Definition graph_to_symm_mat (g : G) : list (list Z) :=
   map (vert_rep_symm g) (nat_inc_list (Z.to_nat SIZE)).
 
+Lemma graph_to_mat_eq:
+  forall (g: G) i j, 0 <= i < SIZE -> 0 <= j < SIZE ->
+    (Znth i (Znth j (graph_to_symm_mat g))) = elabel g (eformat (i,j)).
+Proof.
+intros. unfold graph_to_symm_mat, vert_rep_symm. rewrite Znth_map. rewrite Znth_map. rewrite Znth_map.
+rewrite nat_inc_list_i. rewrite nat_inc_list_i. rewrite eformat_symm; auto.
+lia. lia. rewrite nat_inc_list_Zlength; lia. rewrite Zlength_map.
+all: rewrite nat_inc_list_Zlength; lia.
+Qed.
+
 Lemma graph_to_mat_symmetric:
-  forall (g: G) i j, 0 <= i < j -> j < SIZE ->
+  forall (g: G) i j, 0 <= i < SIZE -> 0 <= j < SIZE ->
     (Znth i (Znth j (graph_to_symm_mat g))) = (Znth j (Znth i (graph_to_symm_mat g))).
 Proof.
 unfold graph_to_symm_mat, vert_rep_symm; intros.
 repeat rewrite Znth_map. repeat rewrite nat_inc_list_i by lia.
-rewrite eformat2; simpl. rewrite eformat1; simpl. auto.
-lia. lia.
+rewrite eformat_symm. auto.
 all: try (rewrite nat_inc_list_Zlength, Z2Nat.id; lia).
 all: rewrite Zlength_map, nat_inc_list_Zlength, Z2Nat.id; lia.
 Qed.
@@ -71,14 +137,14 @@ rewrite Zlength_map, nat_inc_list_Zlength, Z2Nat.id; lia.
 Qed.
 
 Lemma edgeless_vert_rep:
-forall v, 0<=v<SIZE -> vert_rep_symm (@edgeless_graph inf SIZE SIZE_rep) v = list_repeat (Z.to_nat SIZE) inf.
+forall v, 0<=v<SIZE -> vert_rep_symm edgeless_graph' v = list_repeat (Z.to_nat SIZE) inf.
 Proof.
 unfold vert_rep_symm; intros.
 simpl. auto. (*should try to find a better scalable way*)
 Qed.
 
 Lemma edgeless_to_symm_mat:
-graph_to_symm_mat (@edgeless_graph inf SIZE SIZE_rep) = list_repeat (Z.to_nat SIZE) (list_repeat (Z.to_nat SIZE) inf).
+graph_to_symm_mat edgeless_graph' = list_repeat (Z.to_nat SIZE) (list_repeat (Z.to_nat SIZE) inf).
 Proof.
 unfold graph_to_symm_mat.
 simpl. repeat rewrite edgeless_vert_rep; simpl. auto.
